barrier/client.v
@@ -5,22 +5,19 @@ Import uPred.
 Definition client := (let: "b" := newchan '() in wait "b")%L.
 
 Section client.
-  Context {Σ : iFunctorG} `{!heapG Σ} `{!barrierG Σ}.
-  Context (N : namespace) (heapN : namespace).
-
+  Context {Σ : iFunctorG} `{!heapG Σ, !barrierG Σ} (heapN N : namespace).
   Local Notation iProp := (iPropG heap_lang Σ).
 
   Lemma client_safe :
     heapN ⊥ N → heap_ctx heapN ⊑ || client {{ λ _, True }}.
   Proof.
     intros ?. rewrite /client.
-    ewp eapply (newchan_spec N heapN True%I); last done.
+    ewp eapply (newchan_spec heapN N True%I); last done.
     apply sep_intro_True_r; first done.
     apply forall_intro=>l. apply wand_intro_l. rewrite right_id.
     wp_let. etrans; last eapply wait_spec.
-    apply sep_mono_r. apply wand_intro_r. eauto.
+    apply sep_mono_r, wand_intro_r. eauto.
   Qed.
-
 End client.
 
 Section ClosedProofs.
@@ -33,7 +30,7 @@ Section ClosedProofs.
     { (* FIXME Really?? set_solver takes forever on "⊆ ⊤"?!? *)
       by move=>? _. }
     apply wp_strip_pvs, exist_elim=> ?. rewrite and_elim_l.
-    rewrite -(client_safe (nroot .@ "Heap" ) (nroot .@ "Barrier" )) //.
+    rewrite -(client_safe (nroot .@ "Barrier") (nroot .@ "Heap")) //.
     (* This, too, should be automated. *)
     by apply ndot_ne_disjoint.
   Qed.
